Ported lww and orset to new library

lww.fst
@@ -58,6 +58,16 @@ let sim tr s1 =
   s1 = gt tr.l init
 
 let pre_cond_merge ltr l atr a btr b = true
+let pre_cond_merge1 l a b = true
+
+val merge1 : l:s
+           -> a:s
+           -> b:s
+           -> Pure s (requires pre_cond_merge1 l a b)
+                    (ensures (fun r -> (get_id_s a >= get_id_s b ==> r = a) /\
+                                    (get_id_s a < get_id_s b ==> r = b)))
+let merge1 l a b =
+  if (get_id_s a >= get_id_s b) then a else b
 
 val merge : ltr:ae op
           -> l:s
@@ -69,14 +79,11 @@ val merge : ltr:ae op
                              (forall e. mem e atr.l ==> not (mem_id (get_id e) btr.l)) /\
                              (forall e. mem e ltr.l ==> not (mem_id (get_id e) btr.l)) /\
                              (sim ltr l /\ sim (union ltr atr) a /\ sim (union ltr btr) b))
-                    (ensures (fun res -> ((get_id_s a >= get_id_s b) ==> res = a) /\
-                                      ((get_id_s b > get_id_s a) ==> res = b) /\
-                                      (get_id_s res >= get_id_s a /\ get_id_s res >= get_id_s b /\ 
-                                       get_id_s res >= get_id_s l) /\ (res = a \/ res = b)))
+                    (ensures (fun res -> res = merge1 l a b))
 #set-options "--z3rlimit 10000"
 let merge ltr l atr a btr b = 
   assert ((get_id_s a = get_id_s b) ==> (get_id_s l = get_id_s a) /\ (get_id_s l = get_id_s b));
-  if (get_id_s a >= get_id_s b) then a else b
+  merge1 l a b
 
 val lemma : l:list (nat * op)
           -> Lemma (requires unique_id l)
@@ -111,7 +118,6 @@ val prop_oper : tr:ae op
               -> Lemma (requires (sim tr st) /\ (not (mem_id (get_id op) tr.l)) /\
                                 (forall e. mem e tr.l ==> get_id e < get_id op) /\ get_id op > 0)
                       (ensures (sim (append tr op) (app_op st op)))
-
 let prop_oper tr st op = ()
 
 val convergence : tr:ae op
@@ -122,12 +128,16 @@ val convergence : tr:ae op
 let convergence tr a b = ()
 
 instance _ : mrdt s op = {
+  Library.init = init;
   Library.sim = sim;
   Library.pre_cond_op = pre_cond_op;
   Library.app_op = app_op;
   Library.prop_oper = prop_oper;
+  Library.pre_cond_merge1 = pre_cond_merge1;
   Library.pre_cond_merge = pre_cond_merge;
+  Library.merge1 = merge1;
   Library.merge = merge;
   Library.prop_merge = prop_merge;
   Library.convergence = convergence
 }
+
